Wavelet/Compile/Fn/Simulation.lean
@@ -39,6 +39,61 @@ private theorem sim_compile_fn_init
   · simp [compileFn, compileFn.outputs]
   · simp [HasCompiledProcs, compileFn]
 
+private theorem vars_to_chans_init
+  [Arity Op]
+  [InterpConsts V]
+  [DecidableEq χ]
+  (fn : Fn Op χ V m n) :
+    varsToChans ⟨[], []⟩ (Config.init fn) = ChanMap.empty
+  := by
+  funext name
+  simp [varsToChans]
+  cases name <;>
+    simp [Seq.Config.init, VarMap.getVar, VarMap.empty, ChanMap.empty]
+
+theorem sim_compile_fn_preserves_init
+  [Arity Op]
+  [InterpConsts V]
+  [DecidableEq χ]
+  (fn : Fn Op χ V m n)
+  (hwf : fn.AffineVar) :
+    fn.semantics ≲ᵣ[PreservesInit] (compileFn fn).semantics
+  := by
+  apply Lts.SimilaritySt.intro (∃ gs, SimRel gs · ·)
+  · constructor
+    · exact ⟨_, sim_compile_fn_init fn hwf⟩
+    · intros ec pc l ec' hsim hstep
+      replace ⟨_, hsim⟩ := hsim
+      cases h₁ : ec.cont with
+      | init => exact sim_step_init hsim hstep h₁
+      | expr expr =>
+        cases h₂ : expr <;> simp [h₂] at h₁
+        case ret => exact sim_step_ret hsim hstep h₁
+        case tail => exact sim_step_tail hsim hstep h₁
+        case op => exact sim_step_op hsim hstep h₁
+        case br => exact sim_step_br hsim hstep h₁
+  · intros ec pc hsim hinit
+    subst hinit
+    simp [Proc.semantics, Dataflow.Config.init]
+    have ⟨⟨definedVar, pathConds⟩, hsim⟩ := hsim
+    rcases pc with ⟨⟨inputs, outputs, atoms⟩, chans⟩
+    simp
+    have hvars := hsim.vars_to_chans
+    have ⟨_, carryState, _, _, _, hatoms, hcomp, _, hinit, _⟩ := hsim.has_compiled_procs
+    have hinputs := hsim.inputs
+    have houtputs := hsim.outputs
+    simp [Fn.semantics, Seq.Config.init] at hinit
+    have ⟨h₁, _, _, h₂, h₃⟩ := hinit
+    subst h₁ h₂ h₃ hinputs houtputs
+    simp [Fn.semantics, vars_to_chans_init fn] at hvars
+    simp [hvars, compileFn, compileFn.inputs, compileFn.outputs,
+      Fn.semantics, Seq.Config.init]
+    simp [compileFn] at hcomp
+    subst hcomp
+    simp at hatoms
+    rw [hatoms]
+    rfl
+
 /-- Main forward simulation result for `compileFn`. -/
 theorem sim_compile_fn
   [Arity Op]
@@ -46,20 +101,7 @@ theorem sim_compile_fn
   [DecidableEq χ]
   (fn : Fn Op χ V m n)
   (hwf : fn.AffineVar) :
-  fn.semantics ≲ᵣ (compileFn fn).semantics
-  := by
-  apply Lts.Similarity.intro (∃ gs, SimRel gs · ·)
-  constructor
-  · exact ⟨_, sim_compile_fn_init fn hwf⟩
-  · intros ec pc l ec' hsim hstep
-    replace ⟨_, hsim⟩ := hsim
-    cases h₁ : ec.cont with
-    | init => exact sim_step_init hsim hstep h₁
-    | expr expr =>
-      cases h₂ : expr <;> simp [h₂] at h₁
-      case ret => exact sim_step_ret hsim hstep h₁
-      case tail => exact sim_step_tail hsim hstep h₁
-      case op => exact sim_step_op hsim hstep h₁
-      case br => exact sim_step_br hsim hstep h₁
+    fn.semantics ≲ᵣ (compileFn fn).semantics
+  := (sim_compile_fn_preserves_init fn hwf).to_sim
 
 end Wavelet.Compile
